CompCert/cfrontend/Locally.v
@@ -16,16 +16,15 @@ Ltac inv H := inversion H; clear H; subst.
 
 Ltac unfold_locally :=
   unfold locally; unfold hlocally; MonPred.unseal; split; MonPred.unseal; intros i h H;
-  destruct i; inversion H as (H0&H1); clear H; inv H1;
-  clear H0; intros j H; destruct j; clear H;
-  exists emp, heap_empty, heap_empty; repeat split; auto with heap_scope; [intros h H0; inversion_star h H;
-  inversion H1 as (H4&H5); inv H5; clear H4; clear H1; clear H0;
-  rewrite heap_union_empty_l | rewrite heap_union_empty_r; auto].
-
+  destruct i; inversion H as (H1); subst; clear H; intros j H; destruct j; clear H;
+    exists emp, heap_empty, heap_empty; repeat split; auto with heap_scope;
+      [intros h H0; inversion_star h H; inversion H1; clear H0; subst; rewrite heap_union_empty_l
+      | rewrite heap_union_empty_r; auto].
+  
 Lemma locally_base {A} : forall (le : t A), ⊢ locally le (fun le' => emp).
 Proof.
   unfold locally; unfold hlocally; MonPred.unseal; split; MonPred.unseal; intros i h H.
-  intros. inv H.  inv H2. red. split; auto. reflexivity.
+  intros. inv H. reflexivity.
 Qed.
 
 Lemma locally_elim {A} : forall P (le : t A), ⊢ locally le (fun le' => P le') -∗ P le.
@@ -39,10 +38,8 @@ Proof.
   unfold_locally. clear H3. intros j H. destruct j. clear H.
   repeat red. exists (hheap_ctx h1), h1, heap_empty. repeat split; auto with heap_scope.
   red. intros. inversion_star h P. clear H. red in P1. subst.
-  edestruct P2. instantiate (1 := tt). repeat red. exists heap_empty, h0.
-  repeat split; auto with heap_scope.
-  apply map_disjoint_empty_l. rewrite heap_union_empty_l; auto. inversion_star h P.
-  clear H. destruct P4. inv H1. clear P5.
+  edestruct P2. reflexivity. inversion_star h P.
+  clear H. destruct P4. inv H3. clear P5.
   rewrite heap_union_empty_r. rewrite heap_union_empty_r in P3. rewrite heap_union_empty_r in H0.
   apply H. exists h, h1. repeat split; auto. apply H2. intros. erewrite <- H0; auto.
   eapply lookup_union_Some; eauto. apply heap_union_comm; auto. apply map_disjoint_empty_r.
@@ -63,9 +60,9 @@ Proof.
   repeat split; auto with heap_scope.
   repeat red. intros. inversion_star h P. clear H0. red in P1. subst.
   exists h1, h0. repeat split; auto with heap_scope. apply H2.
-  intros. eapply H1.
+  intros. eapply H4.
   eapply lookup_union_Some; eauto with heap_scope.
-  eapply P2. intros. eapply H1. eapply lookup_union_Some; eauto with heap_scope.
+  eapply P2. intros. eapply H4. eapply lookup_union_Some; eauto with heap_scope.
   rewrite heap_union_empty_r; auto. 
 Qed.
 
@@ -75,27 +72,12 @@ Lemma locally_and {A} : forall P R (le : t A),
             locally le (fun le' => P le' ∧ R le').
 Proof.
   unfold locally; unfold hlocally; MonPred.unseal; split; MonPred.unseal; intros i h H;
-  destruct i; inversion H as (H0&H1); clear H; inv H1;
-  clear H0; intros j H; destruct j; clear H.
+  destruct i; inversion H as (H0); clear H; subst. intros j H; destruct j; clear H.
   exists emp, heap_empty, heap_empty; repeat split; auto.
   3 : rewrite heap_union_empty_l; auto.
   all :inversion_star h P; clear H;
-    destruct P2; inv P1; inv H3; clear H2; clear P3; rewrite heap_union_empty_l;
+    destruct P2; inv P1; clear P3; rewrite heap_union_empty_l;
       rewrite heap_union_empty_l in H0. apply (H _ H0). apply (H1 _ H0).
-Qed.
-
-Lemma locally_and_2 {A} : forall P R (le : t A),
-    ⊢locally le (fun le' => P le' ∧ R le') -∗
-     locally le (fun le' => P le') ∧ locally le (fun le' => R le').
-Proof.
-  unfold locally; unfold hlocally; MonPred.unseal; split; MonPred.unseal; intros i h H;
-  destruct i; inversion H as (H0&H1); clear H; inv H1;
-  clear H0; intros j H; destruct j; clear H.
-  exists emp, heap_empty, heap_empty. repeat split; auto.
-  3 : rewrite heap_union_empty_l; auto.
-  all : inversion_star h P; clear H;
-    intros; inv P1; inv H1; clear H0; clear P3; rewrite heap_union_empty_l;
-      rewrite heap_union_empty_l in H; eapply P2 in H; destruct H; auto.
 Qed.
 
 Lemma locally_simpl {A} : forall P (le : t A), ⊢(∀ le', P le') -∗ locally le (fun le' => P le').
@@ -128,7 +110,7 @@ Lemma locally_idempotence {A} : forall P (le : t A),
     ⊢locally le (fun le' => P le') -∗ locally le (fun le' => locally le' (fun le'' => P le'')).
 Proof.
   unfold_locally. intros. apply H2. intros.
-  pose H1. apply H in e.
+  pose H4. apply H0 in e. apply H in H4.
   etransitivity; eauto.
 Qed.
 
@@ -161,13 +143,6 @@ Lemma locally_exists {A B} : forall P (le : t A), ∀ t,
       ⊢locally le (fun le' => P t le') -∗ locally le (fun le' => ∃ (t : B), P t le').
 Proof.
   iIntros. iApply locally_exists'. iExists t0. iFrame.
-Qed.
-
-Lemma locally_exists_sep {A B} : forall P Q (le : t A), ∀ t,
-      ⊢locally le (fun le' => Q t le') -∗ locally le (fun le' => P t le') -∗
-              locally le (fun le' => ∃ (t : B), Q t le' ∗ P t le').
-Proof.
-  iIntros "* HA HB". iApply locally_exists. iApply (locally_sep with "HA HB").
 Qed.
 
 Lemma locally_delete_2 {A} : forall P Q R (le : t A),
